# $Random\ Variable\ \&\ Random\ Vector$

[TOC]

## Define
**Random Variable**:
$$
X: Ω \to \mathbb R  \tag{Random Variable}
$$
a random variable $X$ is a function from a sample space $Ω$ to the real numbers $\mathbb R$.

Symbol:
  - $Ω$: sample space
  - $\mathbb R$: the field of real numbers

- Note  
  event set $\{ζ | X(ζ) ≤ x\}$, shorthand as $\{X ≤ x\}$.

**Random Vector , Multivariate random variable**:
$$
\boldsymbol X = (X_1, ... , X_n)^T  \tag{Random Vector}
$$

## Property
### Probability Mass Function 

- Define 
  for a discrete Random Variable $X$
  $$
  \mathbb P(X = x)
  $$

- Property
  - Nonnegative
    $$
    \mathbb P(X = x) > 0
    $$

  - Sums to 1
    $$
    \sum_i \mathbb P(X = x_i) = 1
    $$

### Cumulative Distribution Function

- Define  
  $$
  \begin{align*}
    F_X(x) &= \mathbb P(X ≤ x)  \\
    F_{\boldsymbol X}(x) &= \mathbb P(X_1 ≤ x_1, ..., X_n ≤ x_n) = \mathbb P(\boldsymbol X ≤ \boldsymbol x)
  \end{align*}
  $$

* Probability Generating Function
  - Define  
    For a discrete random variable $X$ taking values in the non-negative integers $x \in \mathbb Z$, the Probility Generating Function is  
    $$
    G(z) = \mathbb E(z^x) = \sum_{i=0}^\infty z^x \mathbb P(x)
    $$

  - Property
    - $G(1) = 1$
    - $\mathbb P(X = x) = \frac{G^{(k)}(0)}{x!}$
    - $\mathbb E(X) = G'(1)$
    - $Var(X) = G''(1) + G'(1)(1 - G'(1))$ 
    - $\mathbb E(X^k) = \left(z \frac{\partial }{\partial z}\right) G(z)|_{z = 1}$


### Probability Density Function

- Define  
  $$
  \begin{align*}
    f_X(x) &= \frac{\mathrm d F_X(x)}{\mathrm d x}  \\
    f_{\boldsymbol X}(\boldsymbol x) &= \frac{∂^n F_{\boldsymbol X}(x)}{∂ x_1 ... ∂ x_n}  \\
    f_{X_i}(x_i) &= \int_{-\infty}^\infty ... \int_{-\infty}^\infty f_{\boldsymbol X}(\boldsymbol x) \mathrm d x_1 ... \mathrm d x_j ... \mathrm d x_n |_{j ≠ i}  \tag{Marginal Probability Density}
  \end{align*}
  $$

### [Moment](./Moment.md)

### Transformation Between Distributions

For one-to-one mapping of random variables $g: x \to y$ and random vectors $g: \boldsymbol  x \to \boldsymbol  y$, the transformation between distributions is like,
$$
f_Y(y) = \frac{1}{|\frac{\mathrm d y}{\mathrm d x}|} f_X(g^{-1}(y))
$$

$$
f_{\boldsymbol Y}(\boldsymbol y) = \frac{1}{|\det(J_g)|} f_{\boldsymbol X}(g^{-1}(\boldsymbol y))
$$



- Problem: generation of random number
* Mersenne Twister



## Include: Probability Distribution 
### Discrete Probability Distribution 

#### 0-1 distribution ; Bernoulli distribution

- Define  
  It is the discrete probability distribution of a random variable which 
  $$
  \begin{align*}
  \mathbb P(X = 1) &= p  \\
  \mathbb P(X = 0) &= 1 - p
  \end{align*}
  $$

- Property
  | property | value |
  |---|---|
  | Support | $k\in \{0,1\}$ |
  | Probability mass function | $\begin{array}{ll} \mathbb P(X = 1) = p\\ \mathbb P(X = 0) = 1 - p\end{array}$ |
  | Cumulative distribution function | $\mathbb P(X \le x) = \left\{\begin{array}{ll} 0 & \text { if } x<0 \\ 1-p & \text { if } 0 \leq x<1 \\ 1 & \text { if } x \geq 1 \end{array}\right.$ |
  | Mean | $\mathbb E(x) = p$ |
  | Variance | $D(x) = p (1 - p)$ |
  | Skewness | $\frac{1 - 2 p}{\sqrt{p (1 - p)}}$ |
  | Kurtosis | $\frac{1 - 6 p (1 - p)}{p (1 - p)}$ |
  | Entropy | $-p \ln p - (1-p) \ln (1-p)$ |
  |||

#### Binomial distribution 

- Define  
  When n independent Bernoulli trials are performed with the same success probability $p$, the Binomial distribution with parameters $n$ and $p$ is the distribution of $X$, which is the number $n$ of successes.
  $$\mathbb P(X = k) = C^k_n p^k (1-p)^{n-k}$$

- Property  
  | property | value |
  |---|---|
  | Mean | $\mathbb E(x) = n p$ |
  | Variance | $D(x) = n p(1 - p)$ |
  |||

#### Geometric distribution 

- Define  
  $$\mathbb P(X = k) = p (1-p)^{n-1}$$
  描述连续独立重复实验中, 首次成功所进行的实验次数.

- Property
  | property | value |
  |---|---|
  | Mean | $\mathbb E(x) = \frac{1}{p}$ |
  | Variance | $D(x) = \frac{1 - p}{p^2}$ |
  |||

#### Hypergeometric distribution 

- Define  
  $$\mathbb P(X = k) = \frac{C_M^k C_{N_M}^{n-k}}{C_N^n}$$

- Property  
  | property | value |
  |---|---|
  | Mean | $\mathbb E(x) = \frac{n M}{N}$ |
  | Variance | $D(x) = \frac{n M}{N} (1 - \frac{M}{N}) \frac{N - M}{N - 1}$ |
  |||

#### Poisson distribution 

- Define  
  Poisson process： 
  $$\mathbb P(X = k) = \frac{λ^k}{k!} e^{-λ}$$

  2D & n-D Poisson process：
  - the number of events in a region A is distributed $Pois(\lambda · area(A))
  - the numbers of events in disjoint regions are independent of each other.

- Property  
  | property | value |
  |---|---|
  | Mean | $\mathbb E(x) = λ$ |
  | Variance | $D(x) = λ$ |
  |||

- Theorem{Poisson定理}  
  $$\lim_{n \to \infty, p \to 0, λ = n p} \frac{C_M^k C_{N_M}^{n-k}}{C_N^n} = \frac{λ^k}{k!} e^{-λ}$$

### Continuity Probability Distribution 

#### Uniformity distribution 

- Define  
  $$
  \begin{align*}
    f(x) = \left\{\begin{matrix} \frac{1}{b-a} &\quad a < x < b \\ 0 &\quad other \end{matrix}\right.  \\
    F(x) = \left\{\begin{matrix} 0 &\quad x < a \\ \frac{1}{b-a} &\quad a ≤ x < b \\ 1 &\quad b ≤ x \end{matrix}\right.
  \end{align*}
  $$

- Property  
  | property | value |
  |---|---|
  | Mean | $\mathbb E(x) = \frac{a + b}{2}$ |
  | Variance | $D(x) = \frac{(b - a)^2}{12}$ |
  |||

#### Normal distribution 

- Define
  $$
  \begin{align*}
    f_X(x) &= \frac{1}{\sqrt{2 π} \sigma} e^{-\frac{(x - μ)^2}{2 \sigma^2}} \quad; x \in (-\infty, +\infty)  \\
    f_{\boldsymbol X}(\boldsymbol x) &= \frac{1}{(2 π)^{\frac{n}{2}} |\boldsymbol Σ|^{\frac{1}{2}}} e^{-\frac{(\boldsymbol x - \boldsymbol μ)\boldsymbol Σ^{-1}(\boldsymbol x - \boldsymbol μ)^T}{2}} \tag{Multivariate Normal distribution }
  \end{align*}
  $$

  * Standard Normal distribution 
    $$f_X(x) = \frac{1}{\sqrt{2 π}} e^{-\frac{x^2}{2}} \quad; x \in (-\infty, +\infty)$$
    $$μ = 0, \sigma^2 = 1$$

- Property  
  - basic parameters 
    | property | value |
    |---|---|
    | Mean | $\mathbb E(x) = μ$ |
    | Variance | $\begin{array}{ll} D(x) = \sigma^2 \\ D(\boldsymbol x) = \boldsymbol Σ \end{array}$ |
    |||

    - Proof  
      $$
      \begin{align*}
        D(x) &= \frac{1}{(2 π)^{\frac{D}{2}}} \frac{1}{|\boldsymbol Σ|^{\frac{1}{2}}} \sum_{i=1}^D \sum_{j=1}^D \boldsymbol u_i \boldsymbol u_j^T \int e^{-\sum\limits_{k=1}^D \frac{\boldsymbol y_k^2}{2 λ_k}} y_i y_j \mathrm d \boldsymbol y   \\
          &= \frac{1}{(2 π)^{\frac{D}{2}}} \frac{1}{|\boldsymbol Σ|^{\frac{1}{2}}} \sum_{i=1}^D \boldsymbol u_i \boldsymbol u_i^T \int e^{-\sum\limits_{k=1}^D \frac{y_k^2}{2 λ_k}} y_i^2 \mathrm d \boldsymbol y  \tag{$i ≠ j, \boldsymbol u_i \boldsymbol u_j^T=0, \boldsymbol u_i \boldsymbol u_j$ 正交}  \\
          &= \frac{1}{(2 π)^{\frac{D}{2}}} \frac{1}{|\boldsymbol Σ|^{\frac{1}{2}}} \sum_{i=1}^D \boldsymbol u_i \boldsymbol u_i^T \int \prod_{k=1}^D e^{-\frac{y_k^2}{2 λ_k}} y_i^2 \mathrm d \boldsymbol y   \\
          &= \frac{1}{(2 π)^{\frac{D}{2}}} \frac{1}{|\boldsymbol Σ|^{\frac{1}{2}}} \sum_{i=1}^D \boldsymbol u_i \boldsymbol u_i^T \left(\int_{-\infty}^{+\infty} e^{-\frac{y_i^2}{2 λ_i}} y_i^2 \mathrm d y_i × \prod_{k=1, k ≠ i}^D \int_{-\infty}^{+\infty} e^{-\frac{y_X^2}{2 λ_k}} \mathrm d y_k \right)  \tag{积分乘法结合律}  \\
          &= \frac{1}{(2 π)^{\frac{D}{2}}} \frac{1}{|\boldsymbol Σ|^{\frac{1}{2}}} \sum_{i=1}^D \boldsymbol u_i \boldsymbol u_i^T \left((2 π λ_i)^{\frac{1}{2}} · λ_i × \prod_{k=1, k ≠ i}^D(2 π λ_k)^{\frac{1}{2}} \right)  \tag{见下面推导}  \\
          &= \frac{1}{(2 π)^{\frac{D}{2}}} \frac{1}{|\boldsymbol Σ|^{\frac{1}{2}}}  · \left((2 π)^{\frac{D}{2}} \prod_{k=1}^D λ_k \right) · \left(\sum_{i=1}^D \boldsymbol u_i \boldsymbol u_i^T λ_i\right)   \\
          &= \sum_{i=1}^D \boldsymbol u_i \boldsymbol u_i^T λ_i  \tag{$\prod_{k=1}^D λ_k=|\boldsymbol Σ|^{\frac{1}{2}}$}  \\
          &= \boldsymbol Σ
      \end{align*}
      $$

      when $k = i$,
      $$
      \begin{align*}
        \int_{-\infty}^{+\infty} e^{-\frac{y_λ^2}{2 λ_i}} y_i^2 \mathrm d y_i &=(λ_i \sqrt{2 λ_i}) · \int_{-\infty}^{+\infty} \left(\frac{y_i^2}{2 λ_i} \right)^{\frac{1}{2}} e^{-\frac{y_λ^2}{2 λ_i}} \mathrm d \frac{y_i^2}{2 λ_i}   \\
        &= (λ_i \sqrt{2 λ_i}) · 2 Γ(3/2)  \tag{$Γ(z) = \int_0^{+\infty} x^{z-1} e^{-x} \mathrm d x$}  \\
        &= \sqrt{2 π λ_i} · λ_i  \tag{$Γ(3/2) = \frac{\sqrt{π}}{2}$}
      \end{align*}
      $$

      when $k ≠ i$,
      $$
      \begin{align*}
        \int_{-\infty}^{+\infty} e^{-\frac{y_λ^2}{2 λ_k}} \mathrm d y_k &=(\sqrt{\frac{λ_k}{2}}) · \int_{-\infty}^{+\infty} \left(\frac{y_k^2}{2 λ_k} \right)^{-\frac{1}{2}} e^{-\frac{y_λ^2}{2 λ_k}} \mathrm d \frac{y_k^2}{2 λ_k}   \\
        &= \left(\sqrt{\frac{λ_k}{2}}\right) · 2 Γ(\frac{1}{2})  \tag{$Γ(z) = \int_0^{+\infty} x^{z-1} e^{-x} \mathrm d x$}  \\
        &= \sqrt{2 π λ_k}  \tag{$Γ(\frac{1}{2}) = \sqrt{π}$}
      \end{align*}
      $$

  - Conditional Distributions  
    A multivariable $\boldsymbol x$ is partitioned as follows
    $$\boldsymbol x = \left(\begin{matrix}\boldsymbol x_1 \\ \boldsymbol x_2\end{matrix}\right) \sim \mathcal N \left(\left(\begin{matrix}\boldsymbol \mu_1 \\ \boldsymbol \mu_2\end{matrix}\right), \left(\begin{matrix} \boldsymbol \Sigma_{11} & \boldsymbol \Sigma_{12}\\ \boldsymbol \Sigma_{21} & \boldsymbol \Sigma_{22}\end{matrix}\right)\right)$$

    Then the distribution of $\boldsymbol x_1$ conditional on $\boldsymbol x_2 = a$ is still a multivariate normal 
    $$(\boldsymbol x_1\ |\ \boldsymbol x_2 = \boldsymbol a) \sim \mathcal N\left(\boldsymbol \mu_1 + \boldsymbol \Sigma_{12} \boldsymbol \Sigma_{22}^{-1} (\boldsymbol a - \boldsymbol \mu_2), \boldsymbol \Sigma_{11} - \boldsymbol \Sigma_{12} \boldsymbol \Sigma_{22}^{-1} \boldsymbol \Sigma_{21} \right)$$

#### Rayleigh  distribution

- Define  
  $$
    f_X(x) = \frac{x}{σ^2} e^{\frac{-x^2}{2 σ^2}}
  $$

#### $Γ$ distribution 

- Define
  $$
    f(x) = \left\{\begin{matrix} \frac{1}{β^α Γ(α)} x^{a^{-1}} e^{-x / β} &\quad x \in (0, +\infty) \\ 0 &\quad x \in (-\infty, 0] \end{matrix}\right.
  $$
- Property  
  | property | value |
  |---|---|
  | Mean | $\mathbb E(x) = α β$ |
  | Variance | $D(x) = α β^2$ |
  |||

  when $α=1$, $Γ$ distribution 退化为Exponential distribution;  
  when $α=\frac{n}{2}, β=\frac{1}{2}$, $Γ$ distribution 退化为$\chi^2$ distribution.

#### Exponential distribution 

- Define  
  $$f(x) = \left\{\begin{matrix} λ e^{-λ x} &\quad x \in (0, +\infty) \\ 0 &\quad x \in (-\infty, 0] \end{matrix}\right.$$
  $$F(x) = \left\{\begin{matrix} λ 1 - e^{-λ x} &\quad x \in (0, +\infty) \\ 0 &\quad x \in (-\infty, 0] \end{matrix}\right.$$

- Property
  | property | value |
  |---|---|
  | Mean | $\mathbb E(x) = θ$ |
  | Variance | $D(x) = θ^2$ |
  |||

#### $\chi^2$ distribution 

- Define
  $$\frac{1}{2^{\frac{n}{2}} Γ(\frac{n}{2})} x^{\frac{n}{2} - 1} e^{-x / 2}$$

- Property
  | property | value |
  |---|---|
  | Mean | $\mathbb E(x) = n$ |
  | Variance | $D(x) = 2 n$ |
  |||
