* Quartic Function
  - Define
    $$f(x) = \sum_{i=0}^{4} a_i x^i  \tag{Univariate}$$

    $$\begin{align*}
      f(\boldsymbol x) =& \sum_{i_1=1}^{\dim} \sum_{i_2=i_1}^{\dim} \sum_{i_3=i_2}^{\dim} \sum_{i_4=i_3}^{\dim} a_{i_1 i_2 i_3 i_4} 路 x_{i_1} x_{i_2} x_{i_3} x_{i_4} +    \\
      &\sum_{i_1=1}^{\dim} \sum_{i_2=i_1}^{\dim} \sum_{i_3=i_2}^{\dim} b_{i_1 i_2 i_3} 路 x_{i_1} x_{i_2} x_{i_3} +    \\
      &\sum_{i_1=1}^{\dim} \sum_{i_2=i_1}^{\dim} c_{i_1 i_2} 路 x_{i_1} x_{i_2} +    \\
      &\sum_{i_1=0}^{\dim} d_{i_1} x_{i_1} +    \\
      &e  \tag{Multivariate}  \\
      =& \sum_{i_0=0}^{\dim} \sum_{i_1=i_0}^{\dim} \sum_{i_2=i_1}^{\dim} \sum_{i_3=i_2}^{\dim} \sum_{i_4=i_3}^{\dim} a_{i_0 i_1 i_2 i_3 i_4} 路 x_{i_0} x_{i_1} x_{i_2} x_{i_3} x_{i_4}  \quad, x_0 = 1
    \end{align*}$$

  - Property
    * Zero Set of Quartic Function , Quartic Surface
      - Define
      - Property
        - Solution of Univariate Quartic Equation  
          For an Univariate Quartic Equation,
          $$a x^4 + b x^3 + c x^2 + d x + e = 0$$

          The solutions are $r_1, r_2, r_3, r_4$,
          $$\begin{align*}
            r_{i} &= -\frac{b}{4 a} - S \pm \frac{1}{2} \sqrt{-4 S^2 -2 p \pm \frac{q}{S}}  \\
            p & =\frac{8 a c-3 b^2}{8 a^2} \\
            q & =\frac{b^3-4 a b c+8 a^2 d}{8 a^3} \\
            S & =\frac{1}{2} \sqrt{-\frac{2}{3} p+\frac{1}{3 a}\left(Q+\frac{\Delta_0}{Q}\right)} \\
            Q & =\sqrt[3]{\frac{\Delta_1+\sqrt{\Delta_1^2-4 \Delta_0^3}}{2}} \\
            \Delta_0 & =c^2-3 b d+12 a e \\
            \Delta_1 & =2 c^3-9 b c d+27 b^2 e+27 a d^2-72 a c e
          \end{align*}$$

          Or representation by
          $$\begin{align*}
            Q_1 &= c^2 - 3bd + 12e  \\
            Q_2 &= 2c^3 - 9bcd + 27d^2 + 27b^2e - 72ce  \\
            Q_3 &= 8bc - 16d - 2b^3  \\
            Q_4 &= 3b^2 - 8c  \\
            Q_5 &= \sqrt[3]{\frac{Q_2}{2} + \sqrt{\left(\frac{Q_2^2}{4} - Q_1^3\right)}}   \\
            Q_6 &= \frac{Q_1}{Q_5} + Q_5  \\
            Q_7 &= 2\sqrt{\frac{Q_4}{12} + Q_6}   \\
            x_1 &= \frac{-b - Q_7 - \sqrt{4\left(\frac{Q_4}{6} - Q_6 - \frac{Q_3}{Q_7}\right)}}{4} \\
            x_2 &= \frac{-b - Q_7 + \sqrt{4\left(\frac{Q_4}{6} - Q_6 - \frac{Q_3}{Q_7}\right)}}{4} \\
            x_3 &= \frac{-b + Q_7 - \sqrt{4\left(\frac{Q_4}{6} - Q_6 + \frac{Q_3}{Q_7}\right)}}{4} \\
            x_4 &= \frac{-b + Q_7 + \sqrt{4\left(\frac{Q_4}{6} - Q_6 + \frac{Q_3}{Q_7}\right)}}{4}
          \end{align*}$$
      - Include
        * Torus
          - Define  
            $$\{\boldsymbol x \ |\ (R^2 - r^2 + \boldsymbol x^T \boldsymbol x)^2 - 4 R^2 (\boldsymbol x^T \boldsymbol x - x_i^2) = 0\}  \tag{Torus}$$  

        * Tanglecube
          - Define
            $$\left\{\boldsymbol x \ |\ \sum_{i=1}^3 \left(x_i^4 - 5 x_i^2 \right) + 11.8 = 0 \right\}  \tag{Tanglecube}$$   
      